James C - added (and completed) linearization step

FiniteMap.thy
@@ -12,4 +12,59 @@ fun domain_distinct :: "'a \<leadsto> 'b \<Rightarrow> bool" where
   "domain_distinct [] = True"
 | "domain_distinct ((a, b) # ab) = (domain_distinct ab \<and> a \<notin> dom (lookup ab))"
 
+function linearize :: "('a \<rightharpoonup> 'b) \<Rightarrow> 'a \<leadsto> 'b" where
+  "\<not> finite (dom f) \<Longrightarrow> linearize f = undefined"
+| "finite (dom f) \<Longrightarrow> card (dom f) = 0 \<Longrightarrow> linearize f = []"
+| "finite (dom f) \<Longrightarrow> card (dom f) \<noteq> 0 \<Longrightarrow> linearize f = (
+    let x = SOME x. x \<in> dom f
+    in (x, the (f x)) # linearize (f(x := None)))"
+  by atomize_elim auto
+termination
+  proof (relation "measure (card o dom)")
+    show "wf (measure (card \<circ> dom))" by simp
+  next
+    fix f :: "'a \<rightharpoonup> 'b"
+    fix x
+    assume "card (dom f) \<noteq> 0"
+    then obtain y where "y \<in> dom f" by fastforce
+    hence "\<exists>y. y \<in> dom f" by fastforce
+    moreover assume "finite (dom f)"
+    moreover assume "x = (SOME x. x \<in> dom f)"
+    ultimately have "card (dom f - {x}) < card (dom f)" by (metis card_Diff1_less someI_ex)
+    thus "(f(x := None), f) \<in> measure (card \<circ> dom)" by simp
+  qed
+
+lemma [simp]: "finite (dom f) \<Longrightarrow> lookup (linearize f) x = f x"
+  proof (induction f rule: linearize.induct)
+  case 1
+    thus ?case by simp
+  next case 2
+    thus ?case by simp
+  next case (3 f)
+    let ?x = "SOME x. x \<in> dom f"
+    show ?case
+      proof (cases "x = ?x")
+      case True
+        from 3 have "Some (the (f ?x)) = f ?x" 
+          by (metis (mono_tags, lifting) domIff fun_upd_triv linearize.simps(3) 
+              not_Cons_self2 option.collapse someI_ex)
+        with 3 True show ?thesis by (simp add: Let_def)
+      next case False
+        from 3 have "lookup (linearize (f(?x := None))) x = (f(?x := None)) x" by fastforce
+        with 3 False show ?thesis by (simp add: Let_def)
+      qed
+  qed
+
+lemma [simp]: "finite (dom f) \<Longrightarrow> domain_distinct (linearize f)"
+  proof (induction f rule: linearize.induct)
+  case 1
+    thus ?case by simp
+  next case 2
+    thus ?case by simp
+  next case (3 f)
+    let ?x = "SOME x. x \<in> dom f"
+    from 3 have "domain_distinct (linearize (f(?x := None)))" by fastforce
+    with 3 show ?case by (auto simp add: Let_def)
+  qed
+
 end
