TotalCorrectness.thy
@@ -5,32 +5,39 @@ begin
 definition state_convert :: "stack_program \<Rightarrow> stack_state \<Rightarrow> machine_state set" where
   "state_convert \<Pi> \<Sigma>\<^sub>S = {\<Sigma>\<^sub>M | \<Sigma>\<^sub>A \<Sigma>\<^sub>M. 
     \<Sigma>\<^sub>A \<in> StackToAssembly.state_convert \<Sigma>\<^sub>S \<and> 
-      \<Sigma>\<^sub>M \<in> AssemblyToMachine.state_convert (StackToAssembly.program_convert \<Pi>) \<Sigma>\<^sub>A}"
+      \<Sigma>\<^sub>M \<in> AssemblyToMachine.state_convert (linearize (StackToAssembly.program_convert \<Pi>)) \<Sigma>\<^sub>A}"
 
 definition program_convert :: "stack_program \<Rightarrow> machine_program" where
-  "program_convert \<Pi> = AssemblyToMachine.program_convert (StackToAssembly.program_convert \<Pi>)"
+  "program_convert \<Pi> =
+    AssemblyToMachine.program_convert (linearize (StackToAssembly.program_convert \<Pi>))"
 
-theorem total_correctness: "iterate (eval_stack \<Pi>) \<Sigma>\<^sub>S \<Sigma>\<^sub>S' \<Longrightarrow> \<Sigma>\<^sub>M \<in> state_convert \<Pi> \<Sigma>\<^sub>S \<Longrightarrow> 
-    domain_distinct \<Pi> \<Longrightarrow> 
-      \<exists>\<Sigma>\<^sub>M'. \<Sigma>\<^sub>M' \<in> state_convert \<Pi> \<Sigma>\<^sub>S' \<and> iterate (eval_machine (program_convert \<Pi>)) \<Sigma>\<^sub>M \<Sigma>\<^sub>M'"
+theorem total_correctness: "finite (dom \<Pi>) \<Longrightarrow> iterate (eval_stack \<Pi>) \<Sigma>\<^sub>S \<Sigma>\<^sub>S' \<Longrightarrow> 
+  \<Sigma>\<^sub>M \<in> state_convert \<Pi> \<Sigma>\<^sub>S \<Longrightarrow> 
+    \<exists>\<Sigma>\<^sub>M'. \<Sigma>\<^sub>M' \<in> state_convert \<Pi> \<Sigma>\<^sub>S' \<and> iterate (eval_machine (program_convert \<Pi>)) \<Sigma>\<^sub>M \<Sigma>\<^sub>M'"
   proof -
+    assume D: "finite (dom \<Pi>)"
+    hence DL: "domain_distinct (linearize (StackToAssembly.program_convert \<Pi>))" by simp
+    from D have DF: "finite (dom (StackToAssembly.program_convert \<Pi>))" by simp
     assume ES: "iterate (eval_stack \<Pi>) \<Sigma>\<^sub>S \<Sigma>\<^sub>S'"
-    assume "domain_distinct \<Pi>" 
-    hence D: "domain_distinct (StackToAssembly.program_convert \<Pi>)" by simp
     assume "\<Sigma>\<^sub>M \<in> state_convert \<Pi> \<Sigma>\<^sub>S"
     with state_convert_def obtain \<Sigma>\<^sub>A where SA: "\<Sigma>\<^sub>A \<in> StackToAssembly.state_convert \<Sigma>\<^sub>S \<and> 
-      \<Sigma>\<^sub>M \<in> AssemblyToMachine.state_convert (StackToAssembly.program_convert \<Pi>) \<Sigma>\<^sub>A" by blast
+        \<Sigma>\<^sub>M \<in> AssemblyToMachine.state_convert (linearize (StackToAssembly.program_convert \<Pi>)) \<Sigma>\<^sub>A" 
+      by blast
     with ES stack_to_assembly_correct obtain \<Sigma>\<^sub>A' where SA': 
       "\<Sigma>\<^sub>A' \<in> StackToAssembly.state_convert \<Sigma>\<^sub>S' \<and> 
-        iterate (eval_linear_assembly (StackToAssembly.program_convert \<Pi>)) \<Sigma>\<^sub>A \<Sigma>\<^sub>A'" by blast
-    with SA D assembly_to_machine_correct obtain \<Sigma>\<^sub>M' where SM': 
-      "\<Sigma>\<^sub>M' \<in> AssemblyToMachine.state_convert (StackToAssembly.program_convert \<Pi>) \<Sigma>\<^sub>A' \<and> 
-        iterate (eval_machine 
-          (AssemblyToMachine.program_convert (StackToAssembly.program_convert \<Pi>))) \<Sigma>\<^sub>M \<Sigma>\<^sub>M'" by blast
+        iterate (eval_assembly (StackToAssembly.program_convert \<Pi>)) \<Sigma>\<^sub>A \<Sigma>\<^sub>A'" by blast
+    with ES DF linearization_correct have 
+      "iterate (eval_linear_assembly (linearize (StackToAssembly.program_convert \<Pi>))) \<Sigma>\<^sub>A \<Sigma>\<^sub>A'" 
+      by blast
+    with SA DL assembly_to_machine_correct obtain \<Sigma>\<^sub>M' where SM': 
+      "\<Sigma>\<^sub>M' \<in> AssemblyToMachine.state_convert (linearize (StackToAssembly.program_convert \<Pi>)) \<Sigma>\<^sub>A' \<and> 
+        iterate (eval_machine (AssemblyToMachine.program_convert 
+          (linearize (StackToAssembly.program_convert \<Pi>)))) \<Sigma>\<^sub>M \<Sigma>\<^sub>M'" by blast
     with SA' have "\<Sigma>\<^sub>M' \<in> {\<Sigma>\<^sub>M' | \<Sigma>\<^sub>A' \<Sigma>\<^sub>M'. 
       \<Sigma>\<^sub>A' \<in> StackToAssembly.state_convert \<Sigma>\<^sub>S' \<and> 
-        \<Sigma>\<^sub>M' \<in> AssemblyToMachine.state_convert (StackToAssembly.program_convert \<Pi>) \<Sigma>\<^sub>A'}" by blast
-    with SM' have "\<Sigma>\<^sub>M' \<in> state_convert \<Pi> \<Sigma>\<^sub>S' \<and> iterate (eval_machine (program_convert \<Pi>)) \<Sigma>\<^sub>M \<Sigma>\<^sub>M'" 
+        \<Sigma>\<^sub>M' \<in> AssemblyToMachine.state_convert (linearize (StackToAssembly.program_convert \<Pi>)) \<Sigma>\<^sub>A'}" 
+      by blast
+    with SM' have "\<Sigma>\<^sub>M' \<in> state_convert \<Pi> \<Sigma>\<^sub>S' \<and> iterate (eval_machine (program_convert \<Pi>)) \<Sigma>\<^sub>M \<Sigma>\<^sub>M'"
       by (simp add: state_convert_def program_convert_def)
     thus ?thesis by fastforce
   qed
